SeparationLogic/examples/QCP_demos_LLM/kosaraju_rel_proof_manual.v
@@ -55,13 +55,13 @@ Lemma proof_of_dfs1_entail_wit_3_1 : dfs1_entail_wit_3_1.
 Proof. pre_process; cbv [applyf dfs_finish_fromK] in *; Exists timer_v_. Exists vis1_l_. Exists fin_l_; entailer!; lia. Qed.
 
 Lemma proof_of_dfs1_entail_wit_3_2 : dfs1_entail_wit_3_2.
-Proof. Admitted. 
+Proof. right; intros; pre_process; Exists timer_m_2; entailer!; subst v; apply (dfs1_skip_close g_low_level_spec radj_col_l_low_level_spec radj_row_l_low_level_spec u_pre i vis1_m_2 fin_m_2 timer_m_2 X_low_level_spec); [ rewrite <- PreH6; exact PreH9 | split; [ exact PreH17 | rewrite PreH3; exact PreH18 ] | exact PreH1 | exact PreH4 ]. Qed.
 
 Lemma proof_of_dfs1_return_wit_1 : dfs1_return_wit_1.
-Proof. Admitted. 
+Proof. right; intros; pre_process; Exists (timer_m + 1)%Z; entailer!. - destruct PreH2 as [D1 [D2 [D3 [D4 [D5 [D6 [D7 [D8 [D9 D10]]]]]]]]]; apply (dfs1_return_close g_low_level_spec radj_col_l_low_level_spec radj_row_l_low_level_spec u_pre i vis1_m fin_m timer_m X_low_level_spec); [ split; [ exact PreH11 | rewrite PreH3; exact PreH12 ] | exact PreH14 | exact D4 | rewrite <- PreH6; lia | exact PreH4 ]. - unfold csr_wf1, AdjGraphValid in *; destruct PreH2 as [A1 [A2 [A3 [A4 [A5 [A6 [A7 [A8 [A9 A10]]]]]]]]]; destruct A1 as [B1 [B2 [B3 [B4 B5]]]]; repeat (rewrite Zlength_replace_Znth in * |- *); repeat (split; try assumption; try lia; try congruence; try (symmetry; assumption)). Qed.
 
 Lemma proof_of_dfs1_partial_solve_wit_6_pure_split_goal_1 : dfs1_partial_solve_wit_6_pure_split_goal_1.
-Proof. intros; pre_process; cbv [applyf dfs_finish_fromK] in *; entailer!; assert (Hi : (i < csr_hi u_pre radj_row_l_low_level_spec)%Z) by (rewrite <- PreH18; exact PreH21); pose proof (dfs_finish_from_step g_low_level_spec radj_col_l_low_level_spec radj_row_l_low_level_spec u_pre i Hi) as Heq; apply safeExec_proequiv with (c1 := dfs_finish_from g_low_level_spec radj_col_l_low_level_spec radj_row_l_low_level_spec u_pre i); [rewrite PreH30; exact Heq | exact PreH16]. Qed.
+Proof. intros; pre_process; cbv [applyf dfs_finish_fromK] in *; entailer!; subst v; apply (dfs1_recurse_close g_low_level_spec radj_col_l_low_level_spec radj_row_l_low_level_spec u_pre i vis1_m fin_m timer_m X_low_level_spec); [ rewrite <- PreH18; exact PreH21 | split; [ exact PreH29 | rewrite PreH15; exact PreH30 ] | exact PreH13 | exact PreH16 ]. Qed.
 
 Lemma proof_of_dfs1_partial_solve_wit_6_pure_split_goal_2 : dfs1_partial_solve_wit_6_pure_split_goal_2.
 Proof. pre_process; match goal with H : csr_wf1 _ _ _ _ _ |- _ => destruct H | H : csr_wf2 _ _ _ _ _ |- _ => destruct H | _ => idtac end; entailer!; try lia; try congruence; try assumption. Qed.
@@ -70,39 +70,36 @@ Lemma proof_of_dfs1_partial_solve_wit_6_pure : dfs1_partial_solve_wit_6_pure.
 Proof. right; intros. pose proof (proof_of_dfs1_partial_solve_wit_6_pure_split_goal_1) as H1. pose proof (proof_of_dfs1_partial_solve_wit_6_pure_split_goal_2) as H2. unfold dfs1_partial_solve_wit_6_pure_split_goal_1 in H1. unfold dfs1_partial_solve_wit_6_pure_split_goal_2 in H2. apply _derivable1_andp_intros; [ solve [eapply H1; repeat eassumption] | solve [eapply H2; repeat eassumption] ]. Qed.
 
 Lemma proof_of_dfs2_entail_wit_1_split_goal_1 : dfs2_entail_wit_1_split_goal_1.
-Proof. intros; pre_process; entailer!; repeat match goal with H : csr_wf2 _ _ _ _ _ |- _ => destruct H as [C1 [C2 [C3 [C4 [C5 [C6 [C7 [C8 [C9 C10]]]]]]]]] end; intros Hne Hvis; assert (HLu : (0 <= u_pre)%Z) by lia; match goal with |- Znth ?k ?L 0 = _ => assert (HL : (0 <= k < Zlength sid_l_low_level_spec)%Z) by lia; symmetry; rewrite (Znth_replace_neq sid_l_low_level_spec k u_pre (Znth root_pre sid_l_low_level_spec 0) 0 HL HLu Hne); reflexivity end. Qed.
+Proof. intros; pre_process. repeat match goal with H : csr_wf2 _ _ _ _ _ |- _ => destruct H as [C1 [C2 [C3 [C4 [C5 [C6 [C7 [C8 [C9 C10]]]]]]]]] end. assert (HLu : (0 <= u_pre < Zlength vis2_l_low_level_spec)%Z) by lia. assert (HL0 : (0 <= 0 < Zlength vis2_l_low_level_spec)%Z) by lia. assert (HLn : (0 <= n_pre - 1 < Zlength vis2_l_low_level_spec)%Z) by lia. entailer!. all: intros Hv; match goal with | |- (Znth ?k (replace_Znth ?j 1 ?L) 0 <> 0) => assert (HLk : (0 <= k < Zlength L)%Z) by lia; destruct (Z.eqb k j) eqn:E; [ apply Z.eqb_eq in E; subst j; rewrite (Znth_replace_eq L k 1 0 HLk); lia | apply Z.eqb_neq in E; rewrite (Znth_replace_neq L k j 1 0 HLk (proj1 (HLu)) E); exact Hv ] end. Qed.
 
 Lemma proof_of_dfs2_entail_wit_1_split_goal_2 : dfs2_entail_wit_1_split_goal_2.
-Proof. intros; pre_process; entailer!; repeat match goal with H : csr_wf2 _ _ _ _ _ |- _ => destruct H as [C1 [C2 [C3 [C4 [C5 [C6 [C7 [C8 [C9 C10]]]]]]]]] end; intros Hvis; assert (HLu : (0 <= u_pre < Zlength vis2_l_low_level_spec)%Z) by lia; match goal with |- Znth ?k (replace_Znth ?j 1 ?L) 0 <> 0 => assert (HL : (0 <= k < Zlength vis2_l_low_level_spec)%Z) by lia; destruct (Z.eqb k j) eqn:E; [ apply Z.eqb_eq in E; rewrite <- E; rewrite (Znth_replace_eq vis2_l_low_level_spec k 1 0 HL); lia | apply Z.eqb_neq in E; rewrite (Znth_replace_neq vis2_l_low_level_spec k j 1 0 HL (proj1 HLu) E); exact Hvis ] end. Qed.
+Proof. intros; pre_process; entailer!; repeat match goal with H : csr_wf2 _ _ _ _ _ |- _ => destruct H as [C1 [C2 [C3 [C4 [C5 [C6 [C7 [C8 [C9 C10]]]]]]]]] end; assert (HLu : (0 <= u_pre < Zlength vis2_l_low_level_spec)%Z) by lia; assert (HLr : (0 <= root_pre < Zlength vis2_l_low_level_spec)%Z) by lia; destruct (Z.eqb root_pre u_pre) eqn:E; [ apply Z.eqb_eq in E; rewrite E; rewrite (Znth_replace_eq vis2_l_low_level_spec u_pre 1 0 HLu); lia | apply Z.eqb_neq in E; rewrite (Znth_replace_neq vis2_l_low_level_spec root_pre u_pre 1 0 HLr (proj1 HLu) E); assumption ]. Qed.
 
 Lemma proof_of_dfs2_entail_wit_1_split_goal_3 : dfs2_entail_wit_1_split_goal_3.
-Proof. intros; pre_process; entailer!; match goal with H : csr_wf2 _ _ _ _ _ |- _ => destruct H as [C1 [C2 [C3 [C4 [C5 [C6 [C7 [C8 [C9 C10]]]]]]]]] end; assert (HLu : (0 <= u_pre < Zlength vis2_l_low_level_spec)%Z) by lia; assert (HLr : (0 <= root_pre < Zlength vis2_l_low_level_spec)%Z) by lia; destruct (Z.eqb root_pre u_pre) eqn:E; [ apply Z.eqb_eq in E; rewrite E; rewrite (Znth_replace_eq vis2_l_low_level_spec u_pre 1 0 HLu); lia | apply Z.eqb_neq in E; rewrite (Znth_replace_neq vis2_l_low_level_spec root_pre u_pre 1 0 HLr (proj1 HLu) E); assumption ]. Qed.
+Proof. intros; pre_process; entailer!; repeat match goal with H : csr_wf2 _ _ _ _ _ |- _ => destruct H as [C1 [C2 [C3 [C4 [C5 [C6 [C7 [C8 [C9 C10]]]]]]]]] end; assert (HLu : (0 <= u_pre < Zlength sid_l_low_level_spec)%Z) by lia; assert (HLr : (0 <= root_pre < Zlength sid_l_low_level_spec)%Z) by lia; destruct (Z.eqb root_pre u_pre) eqn:E; [ apply Z.eqb_eq in E; subst u_pre; reflexivity | apply Z.eqb_neq in E; rewrite (Znth_replace_eq sid_l_low_level_spec u_pre (Znth root_pre sid_l_low_level_spec 0) 0 HLu); rewrite (Znth_replace_neq sid_l_low_level_spec root_pre u_pre (Znth root_pre sid_l_low_level_spec 0) 0 HLr (proj1 HLu) E); reflexivity ]. Qed.
 
 Lemma proof_of_dfs2_entail_wit_1_split_goal_4 : dfs2_entail_wit_1_split_goal_4.
-Proof. intros; pre_process; entailer!; match goal with H : csr_wf2 _ _ _ _ _ |- _ => destruct H as [C1 [C2 [C3 [C4 [C5 [C6 [C7 [C8 [C9 C10]]]]]]]]] end; assert (HLu : (0 <= u_pre < Zlength sid_l_low_level_spec)%Z) by lia; assert (HLr : (0 <= root_pre < Zlength sid_l_low_level_spec)%Z) by lia; rewrite (Znth_replace_eq sid_l_low_level_spec u_pre (Znth root_pre sid_l_low_level_spec 0) 0 HLu); destruct (Z.eqb root_pre u_pre) eqn:E; [ apply Z.eqb_eq in E; rewrite E; rewrite (Znth_replace_eq sid_l_low_level_spec u_pre (Znth u_pre sid_l_low_level_spec 0) 0 HLu); reflexivity | apply Z.eqb_neq in E; rewrite (Znth_replace_neq sid_l_low_level_spec root_pre u_pre (Znth root_pre sid_l_low_level_spec 0) 0 HLr PreH5 E); reflexivity ]. Qed.
+Proof. intros; pre_process; entailer!; repeat match goal with H : csr_wf2 _ _ _ _ _ |- _ => destruct H as [C1 [C2 [C3 [C4 [C5 [C6 [C7 [C8 [C9 C10]]]]]]]]] end; assert (HLu : (0 <= u_pre < Zlength vis2_l_low_level_spec)%Z) by lia; rewrite (Znth_replace_eq vis2_l_low_level_spec u_pre 1 0 HLu); lia. Qed.
 
 Lemma proof_of_dfs2_entail_wit_1_split_goal_5 : dfs2_entail_wit_1_split_goal_5.
-Proof. intros; pre_process; entailer!; match goal with H : csr_wf2 _ _ _ _ _ |- _ => destruct H as [C1 [C2 [C3 [C4 [C5 [C6 [C7 [C8 [C9 C10]]]]]]]]] end; assert (HLu : (0 <= u_pre < Zlength vis2_l_low_level_spec)%Z) by lia; rewrite (Znth_replace_eq vis2_l_low_level_spec u_pre 1 0 HLu); lia. Qed.
+Proof. intros; pre_process; match goal with H : csr_wf2 _ _ _ _ _ |- _ => destruct H as [C1 [C2 [C3 [C4 [C5 [C6 [C7 [C8 [C9 C10]]]]]]]]] end; assert (Hb : (0 <= u_pre < adj_verts g_low_level_spec)%Z) by lia; pose proof (C7 u_pre Hb); cbv [csr_lo csr_hi] in *; entailer!; lia. Qed.
 
 Lemma proof_of_dfs2_entail_wit_1_split_goal_6 : dfs2_entail_wit_1_split_goal_6.
-Proof. pre_process. match goal with H : csr_wf2 _ _ _ _ _ |- _ => destruct H as [C1 [C2 [C3 [C4 [C5 [C6 [C7 [C8 [C9 C10]]]]]]]]] end. assert (Hb : (0 <= u_pre < adj_verts g_low_level_spec)%Z) by lia. pose proof (C6 u_pre Hb) as Hlo. pose proof (C7 u_pre Hb) as Hhi. pose proof (C9 u_pre Hb) as Hmon. cbv [csr_lo csr_hi] in *. entailer!; lia. Qed.
-
-Lemma proof_of_dfs2_entail_wit_1_split_goal_7 : dfs2_entail_wit_1_split_goal_7.
 Proof. intros; pre_process; match goal with H : csr_wf2 _ _ _ _ _ |- _ => destruct H as [C1 [C2 [C3 [C4 [C5 [C6 [C7 [C8 [C9 C10]]]]]]]]] end; assert (Hb : (0 <= u_pre < adj_verts g_low_level_spec)%Z) by lia; pose proof (C9 u_pre Hb); cbv [csr_lo csr_hi] in *; entailer!; lia. Qed.
 
-Lemma proof_of_dfs2_entail_wit_1_split_goal_8 : dfs2_entail_wit_1_split_goal_8.
+Lemma proof_of_dfs2_entail_wit_1_split_goal_7 : dfs2_entail_wit_1_split_goal_7.
 Proof. intros; pre_process; match goal with H : csr_wf2 _ _ _ _ _ |- _ => destruct H as [C1 [C2 [C3 [C4 [C5 [C6 [C7 [C8 [C9 C10]]]]]]]]] end; assert (Hb : (0 <= u_pre < adj_verts g_low_level_spec)%Z) by lia; pose proof (C6 u_pre Hb); cbv [csr_lo csr_hi] in *; entailer!; lia. Qed.
 
+Lemma proof_of_dfs2_entail_wit_1_split_goal_8 : dfs2_entail_wit_1_split_goal_8.
+Proof. intros; pre_process; match goal with H : csr_wf2 _ _ _ _ _ |- _ => destruct H as [C1 [C2 [C3 [C4 [C5 [C6 [C7 [C8 [C9 C10]]]]]]]]] end; cbv [csr_lo csr_hi]; entailer!; reflexivity. Qed.
+
 Lemma proof_of_dfs2_entail_wit_1_split_goal_9 : dfs2_entail_wit_1_split_goal_9.
-Proof. pre_process; match goal with H : csr_wf1 _ _ _ _ _ |- _ => destruct H | H : csr_wf2 _ _ _ _ _ |- _ => destruct H | _ => idtac end; entailer!; try lia; try congruence; try assumption. Qed.
+Proof. intros; pre_process; match goal with H : csr_wf2 _ _ _ _ _ |- _ => destruct H as [C1 [C2 [C3 [C4 [C5 [C6 [C7 [C8 [C9 C10]]]]]]]]] end; cbv [csr_lo csr_hi]; entailer!; reflexivity. Qed.
 
 Lemma proof_of_dfs2_entail_wit_1_split_goal_10 : dfs2_entail_wit_1_split_goal_10.
-Proof. intros; pre_process; entailer!; match goal with H : csr_wf2 _ _ _ _ _ |- _ => destruct H as [C1 [C2 [C3 [C4 [C5 [C6 [C7 [C8 [C9 C10]]]]]]]]] end; unfold csr_wf2 in *; repeat (rewrite Zlength_replace_Znth in * |- *); repeat (split; try assumption; try lia; try congruence). Qed.
-
-Lemma proof_of_dfs2_entail_wit_1_split_goal_11 : dfs2_entail_wit_1_split_goal_11.
 Proof. Admitted. 
 
-Lemma proof_of_dfs2_entail_wit_1_split_goal_12 : dfs2_entail_wit_1_split_goal_12.
+Lemma proof_of_dfs2_entail_wit_1_split_goal_11 : dfs2_entail_wit_1_split_goal_11.
 Proof. intros; pre_process; entailer!; match goal with H : csr_wf2 _ _ _ _ _ |- _ => destruct H as [C1 [C2 [C3 [C4 [C5 [C6 [C7 [C8 [C9 C10]]]]]]]]] end; unfold csr_wf2 in *; repeat (rewrite Zlength_replace_Znth in * |- *); repeat (split; try assumption; try lia; try congruence). Qed.
 
 Lemma proof_of_dfs2_entail_wit_1 : dfs2_entail_wit_1.
@@ -121,13 +118,13 @@ Lemma proof_of_dfs2_entail_wit_2 : dfs2_entail_wit_2.
 Proof. right; intros. pose proof (proof_of_dfs2_entail_wit_2_split_goal_1) as H1. pose proof (proof_of_dfs2_entail_wit_2_split_goal_2) as H2. pose proof (proof_of_dfs2_entail_wit_2_split_goal_3) as H3. unfold dfs2_entail_wit_2_split_goal_1 in H1. unfold dfs2_entail_wit_2_split_goal_2 in H2. unfold dfs2_entail_wit_2_split_goal_3 in H3. apply _derivable1_andp_intros; [ apply _derivable1_andp_intros; [ apply _derivable1_andp_intros; [ solve [eapply H1; repeat eassumption] | solve [eapply H2; repeat eassumption] ] | solve [eapply H3; repeat eassumption] ] | pre_process; entailer! ]. Qed.
 
 Lemma proof_of_dfs2_entail_wit_3_1_split_goal_1 : dfs2_entail_wit_3_1_split_goal_1.
-Proof. intros; pre_process; entailer!; try lia; try congruence; try assumption. Qed.
+Proof. Admitted. 
 
 Lemma proof_of_dfs2_entail_wit_3_1_split_goal_2 : dfs2_entail_wit_3_1_split_goal_2.
-Proof. intros; pre_process; entailer!; [ destruct (Z.eqb lo i) eqn:E; [ apply Z.eqb_eq in E; rewrite E; rewrite <- PreH31; exact PreH4 | apply Z.eqb_neq in E; match goal with H : csr_wf2 _ _ _ _ _ |- _ => destruct H as [C1 [C2 [C3 [C4 [C5 [C6 [C7 [C8 [C9 C10]]]]]]]]] end; assert (Hlli : (lo <= lo < i)%Z) by lia; assert (Hblo : (0 <= lo < m_of fadj_row_l_low_level_spec)%Z) by lia; destruct (C8 lo Hblo) as [Hlo' Hhi']; assert (Hw : (0 <= Znth lo fadj_col_l_low_level_spec 0 < n_pre)%Z) by lia; exact (PreH6 (Znth lo fadj_col_l_low_level_spec 0) Hw (PreH25 lo Hlli)) ] | replace (i + 1 - 1)%Z with i by lia; rewrite <- PreH31; exact PreH4 ]. Qed.
+Proof. intros; pre_process. match goal with H : csr_wf2 _ _ _ _ _ |- _ => destruct H as [C1 [C2 [C3 [C4 [C5 [C6 [C7 [C8 [C9 C10]]]]]]]]] end. entailer!. - destruct (Z.eqb lo i) eqn:E; [ apply Z.eqb_eq in E; rewrite E; rewrite <- PreH30; exact PreH4 | apply Z.eqb_neq in E; assert (Hlli : (lo <= lo < i)%Z) by lia; pose proof (PreH24 lo Hlli) as Hsc; apply (PreH6 (Znth lo fadj_col_l_low_level_spec 0)); [ assert (Hblo : (0 <= lo < m_of fadj_row_l_low_level_spec)%Z) by lia; pose proof (C8 lo Hblo) as Hw; rewrite PreH2 in Hw; exact Hw | exact Hsc ] ]. - replace (i + 1 - 1)%Z with i by lia; rewrite <- PreH30; exact PreH4. Qed.
 
 Lemma proof_of_dfs2_entail_wit_3_1_split_goal_3 : dfs2_entail_wit_3_1_split_goal_3.
-Proof. intros; pre_process; entailer!. pose proof (PreH7 u_pre (conj PreH18 PreH19) PreH23) as Hu. pose proof (PreH7 root_pre (conj PreH20 PreH21) PreH26) as Hr. lia. Qed.
+Proof. Admitted. 
 
 Lemma proof_of_dfs2_entail_wit_3_1_split_goal_4 : dfs2_entail_wit_3_1_split_goal_4.
 Proof. pre_process; match goal with H : csr_wf1 _ _ _ _ _ |- _ => destruct H | H : csr_wf2 _ _ _ _ _ |- _ => destruct H | _ => idtac end; entailer!; try lia; try congruence; try assumption. Qed.
@@ -139,40 +136,31 @@ Lemma proof_of_dfs2_entail_wit_3_1 : dfs2_entail_wit_3_1.
 Proof. Admitted. 
 
 Lemma proof_of_dfs2_entail_wit_3_2_split_goal_1 : dfs2_entail_wit_3_2_split_goal_1.
-Proof. intros; pre_process; entailer!; [ destruct (Z.eqb lo i) eqn:E; [ apply Z.eqb_eq in E; rewrite E; rewrite <- PreH25; exact PreH1 | apply Z.eqb_neq in E; assert (Hlli : (lo <= lo < i)%Z) by lia; exact (PreH19 lo Hlli) ] | replace (i + 1 - 1)%Z with i by lia; rewrite <- PreH25; exact PreH1 ]. Qed.
+Proof. Admitted. 
 
 Lemma proof_of_dfs2_entail_wit_3_2_split_goal_2 : dfs2_entail_wit_3_2_split_goal_2.
-Proof. intros; pre_process; entailer!; apply (dfs2_skip_close g_low_level_spec fadj_col_l_low_level_spec fadj_row_l_low_level_spec root_pre u_pre i vis2_m_2 sid_m_2 root_v_low_level_spec X_low_level_spec); [ rewrite <- PreH7; exact PreH10 | rewrite <- PreH25; lia | rewrite <- PreH25; exact PreH1 | exact PreH5 ]. Qed.
+Proof. intros; pre_process. entailer!. - destruct (Z.eqb lo i) eqn:E; [ apply Z.eqb_eq in E; rewrite E; rewrite <- PreH25; exact PreH1 | apply Z.eqb_neq in E; assert (Hlli : (lo <= lo < i)%Z) by lia; exact (PreH19 lo Hlli) ]. - replace (i + 1 - 1)%Z with i by lia; rewrite <- PreH25; exact PreH1. Qed.
+
+Lemma proof_of_dfs2_entail_wit_3_2_split_goal_3 : dfs2_entail_wit_3_2_split_goal_3.
+Proof. Admitted. 
 
 Lemma proof_of_dfs2_entail_wit_3_2 : dfs2_entail_wit_3_2.
-Proof. right; intros; pre_process; entailer!. all: repeat (first [ match goal with | Hvi : ?v = Znth ?ii ?fc 0, Hvisv : Znth ?v ?vis 0 <> 0 |- Znth (Znth (?ii + 1 - 1)%Z ?fc 0) ?vis 0 <> 0 => replace (ii + 1 - 1)%Z with ii by lia; rewrite <- Hvi; exact Hvisv end | (eapply dfs2_scanned_lo_close; [ match goal with H : forall j, ((?lo <= j)%Z /\ (j < ?i)%Z) -> Znth (Znth j ?fc 0) ?vis 0 <> 0 |- _ => exact H end | lia | match goal with H : ?v = Znth ?i ?fc 0 |- _ => exact H end | match goal with H : Znth ?v ?vis 0 <> 0 |- Znth ?v ?vis 0 <> 0 => exact H end ]) | (apply dfs2_skip_close; [ match goal with H1 : ?i < ?hi, H2 : ?hi = csr_hi ?u ?fr |- _ => rewrite <- H2; exact H1 end | match goal with H : ?v = Znth ?i ?fc 0 |- _ => rewrite <- H; lia end | match goal with H : ?v = Znth ?i ?fc 0 |- _ => rewrite <- H; match goal with H2 : Znth ?v ?vis 0 <> 0 |- _ => exact H2 end end | match goal with H : safeExec (pre_dfs2 ?g ?fc ?fr ?vis ?sid ?rv) (dfs_scc_from ?g ?fc ?fr ?root ?u ?i) ?X |- _ => exact H end ]) | split | assumption | lia | congruence | entailer! ]). Qed.
+Proof. Admitted. 
 
 Lemma proof_of_dfs2_return_wit_1_split_goal_1 : dfs2_return_wit_1_split_goal_1.
-Proof. Admitted. 
-
-Lemma proof_of_dfs2_return_wit_1_split_goal_2 : dfs2_return_wit_1_split_goal_2.
-Proof. intros; pre_process; entailer!; apply (dfs2_return_close g_low_level_spec fadj_col_l_low_level_spec fadj_row_l_low_level_spec root_pre u_pre i vis2_m sid_m root_v_low_level_spec X_low_level_spec);
-  [ exact PreH2
-  | exact PreH3
-  | exact PreH17
-  | exact PreH18
-  | rewrite <- PreH6; exact PreH19
-  | split; [ exact PreH12 | rewrite PreH4; exact PreH13 ]
-  | split; [ exact PreH14 | rewrite PreH4; exact PreH15 ]
-  | rewrite <- PreH7; lia
-  | exact PreH5 ]. Qed.
+Proof. intros; pre_process; entailer!; apply (dfs2_return_close g_low_level_spec fadj_col_l_low_level_spec fadj_row_l_low_level_spec root_pre u_pre i vis2_m sid_m root_v_low_level_spec X_low_level_spec); [ rewrite <- PreH7; lia | exact PreH5 ]. Qed.
 
 Lemma proof_of_dfs2_return_wit_1 : dfs2_return_wit_1.
-Proof. Admitted. 
+Proof. right; intros. pose proof (proof_of_dfs2_return_wit_1_split_goal_1) as H1. unfold dfs2_return_wit_1_split_goal_1 in H1. apply _derivable1_andp_intros; [ eapply H1; repeat eassumption | pre_process; entailer! ]. Qed.
 
 Lemma proof_of_dfs2_partial_solve_wit_8_pure_split_goal_1 : dfs2_partial_solve_wit_8_pure_split_goal_1.
-Proof. intros; pre_process; entailer!; rewrite PreH39; apply (dfs2_recurse_close g_low_level_spec fadj_col_l_low_level_spec fadj_row_l_low_level_spec root_pre u_pre i vis2_m sid_m root_v_low_level_spec X_low_level_spec); [ rewrite <- PreH21; exact PreH24 | rewrite <- PreH39; lia | rewrite <- PreH39; exact PreH15 | exact PreH19 ]. Qed.
+Proof. intros; pre_process; entailer!; subst v; apply (dfs2_recurse_close g_low_level_spec fadj_col_l_low_level_spec fadj_row_l_low_level_spec root_pre u_pre i vis2_m sid_m root_v_low_level_spec X_low_level_spec); [ rewrite <- PreH21; exact PreH24 | split; [ exact PreH37 | rewrite PreH18; exact PreH38 ] | exact PreH15 | exact PreH19 ]. Qed.
 
 Lemma proof_of_dfs2_partial_solve_wit_8_pure : dfs2_partial_solve_wit_8_pure.
 Proof. right; intros. pose proof (proof_of_dfs2_partial_solve_wit_8_pure_split_goal_1) as H1. unfold dfs2_partial_solve_wit_8_pure_split_goal_1 in H1. eapply H1; repeat eassumption. Qed.
 
 Lemma proof_of_dfs2_derive_bind_spec_by_low_level_spec : dfs2_derive_bind_spec_by_low_level_spec.
-Proof. intros; pre_process. apply safeExec_bind in H2 as (X_low_level_spec & Hsafe_first & Hsafe_cont). Exists g_bind_spec. Exists fadj_col_l_bind_spec. Exists fadj_row_l_bind_spec. Exists vis2_l_bind_spec. Exists sid_l_bind_spec. Exists root_v_bind_spec. Exists X_low_level_spec. split_pure_spatial. - cancel (IntArray.full fadj_col_pre (m_of fadj_row_l_bind_spec) fadj_col_l_bind_spec). cancel (IntArray.full fadj_row_pre (n_pre + 1) fadj_row_l_bind_spec). cancel (IntArray.full vis2_pre n_pre vis2_l_bind_spec). cancel (IntArray.full sid_pre n_pre sid_l_bind_spec). apply derivable1_wand_sepcon_adjoint. Intros vis2_l__2 sid_l__2. Exists vis2_l__2. Exists sid_l__2. split_pure_spatial. + cancel (IntArray.full fadj_col_pre (m_of fadj_row_l_bind_spec) fadj_col_l_bind_spec). cancel (IntArray.full fadj_row_pre (n_pre + 1) fadj_row_l_bind_spec). cancel (IntArray.full vis2_pre n_pre vis2_l__2). cancel (IntArray.full sid_pre n_pre sid_l__2). + split_pures; dump_pre_spatial. exact H2. exact H1. unfold applyf. apply (Hsafe_cont (pre_dfs2 g_bind_spec fadj_col_l_bind_spec fadj_row_l_bind_spec vis2_l__2 sid_l__2 root_v_bind_spec) tt). exact H10. exact H11. exact H12. exact H13. exact H14. - split_pures; dump_pre_spatial. exact H. exact H0. exact H1. exact Hsafe_first. exact H3. exact H4. exact H5. exact H6. exact H7. exact H8. Qed.
+Proof. intros; pre_process. apply safeExec_bind in H2 as (X_low_level_spec & Hsafe_first & Hsafe_cont). Exists g_bind_spec. Exists fadj_col_l_bind_spec. Exists fadj_row_l_bind_spec. Exists vis2_l_bind_spec. Exists sid_l_bind_spec. Exists root_v_bind_spec. Exists X_low_level_spec. split_pure_spatial. - cancel (IntArray.full fadj_col_pre (m_of fadj_row_l_bind_spec) fadj_col_l_bind_spec). cancel (IntArray.full fadj_row_pre (n_pre + 1) fadj_row_l_bind_spec). cancel (IntArray.full vis2_pre n_pre vis2_l_bind_spec). cancel (IntArray.full sid_pre n_pre sid_l_bind_spec). apply derivable1_wand_sepcon_adjoint. Intros vis2_l__2 sid_l__2. Exists vis2_l__2. Exists sid_l__2. split_pure_spatial. + cancel (IntArray.full fadj_col_pre (m_of fadj_row_l_bind_spec) fadj_col_l_bind_spec). cancel (IntArray.full fadj_row_pre (n_pre + 1) fadj_row_l_bind_spec). cancel (IntArray.full vis2_pre n_pre vis2_l__2). cancel (IntArray.full sid_pre n_pre sid_l__2). + split_pures; dump_pre_spatial. exact H2. exact H1. unfold applyf. apply (Hsafe_cont (pre_dfs2 g_bind_spec fadj_col_l_bind_spec fadj_row_l_bind_spec vis2_l__2 sid_l__2 root_v_bind_spec) tt). exact H10. exact H11. exact H12. exact H13. - split_pures; dump_pre_spatial. exact H. exact H0. exact H1. exact Hsafe_first. exact H3. exact H4. exact H5. exact H6. exact H7. exact H8. Qed.
 
 Lemma proof_of_dfs1_derive_bind_spec_by_low_level_spec : dfs1_derive_bind_spec_by_low_level_spec.
 Proof. intros; pre_process. apply safeExec_bind in H1 as (X_low_level_spec & Hsafe_first & Hsafe_cont). Exists g_bind_spec. Exists radj_col_l_bind_spec. Exists radj_row_l_bind_spec. Exists vis1_l_bind_spec. Exists fin_l_bind_spec. Exists timer_v_bind_spec. Exists X_low_level_spec. split_pure_spatial. - cancel (IntArray.full radj_col_pre (m_of radj_row_l_bind_spec) radj_col_l_bind_spec). cancel (IntArray.full radj_row_pre (n_pre + 1) radj_row_l_bind_spec). cancel (IntArray.full vis1_pre n_pre vis1_l_bind_spec). cancel (IntArray.full fin_pre n_pre fin_l_bind_spec). cancel (IntArray.full timer_p_pre 1 (timer_v_bind_spec :: nil)). apply derivable1_wand_sepcon_adjoint. Intros timer_v__2 vis1_l__2 fin_l__2. Exists timer_v__2. Exists vis1_l__2. Exists fin_l__2. split_pure_spatial. + cancel (IntArray.full radj_col_pre (m_of radj_row_l_bind_spec) radj_col_l_bind_spec). cancel (IntArray.full radj_row_pre (n_pre + 1) radj_row_l_bind_spec). cancel (IntArray.full vis1_pre n_pre vis1_l__2). cancel (IntArray.full fin_pre n_pre fin_l__2). cancel (IntArray.full timer_p_pre 1 (timer_v__2 :: nil)). + split_pures; dump_pre_spatial. exact H1. exact H0. unfold applyf. apply (Hsafe_cont (pre_dfs1 g_bind_spec radj_col_l_bind_spec radj_row_l_bind_spec vis1_l__2 fin_l__2 timer_v__2) tt). exact H9. exact H10. exact H11. - split_pures; dump_pre_spatial. exact H. exact H0. exact Hsafe_first. exact H2. exact H3. exact H4. exact H5. exact H6. exact H7. Qed.
